refactored

Simple_Firewall/SimpleFw_Compliance.thy
@@ -1,5 +1,6 @@
 theory SimpleFw_Compliance
-imports SimpleFw_Semantics "../Primitive_Matchers/IPPortIfaceSpace_Matcher" "../Semantics_Ternary" "../Output_Format/Negation_Type_Matching" "../Bitmagic/Numberwang_Ln"
+imports SimpleFw_Semantics "../Primitive_Matchers/IPPortIfaceSpace_Matcher" "../Semantics_Ternary"
+        "../Output_Format/Negation_Type_Matching" "../Bitmagic/Numberwang_Ln"
 begin
 
 fun ipv4_word_netmask_to_ipt_ipv4range :: "(ipv4addr \<times> nat) \<Rightarrow> ipt_ipv4range" where
@@ -42,7 +43,7 @@ apply(simp_all add: bunch_of_lemmata_about_matches)
 done
 
 (*TODO: smelly duplication*)
-lemma matches_Src_simple_match: "matches (ipportiface_matcher, \<alpha>) (negation_type_to_match_expr (\<lambda>x. ipportiface_rule_match.Src (ipv4_word_netmask_to_ipt_ipv4range x)) ip) a p \<longleftrightarrow>
+lemma matches_Src_simple_match: "matches (ipportiface_matcher, \<alpha>) (negation_type_to_match_expr (\<lambda>x. Src (ipv4_word_netmask_to_ipt_ipv4range x)) ip) a p \<longleftrightarrow>
   simple_match_ip ip (p_src p)"
 apply(cases ip)
  apply(rename_tac i_ip)
@@ -56,7 +57,7 @@ apply(rename_tac iip n)
 apply(simp add: matches_case_ternaryvalue_tuple split: ternaryvalue.split)
 apply(simp add: bunch_of_lemmata_about_matches bool_to_ternary_simps ipv4addr_of_dotteddecimal_dotteddecimal_of_ipv4addr)
 done
-lemma matches_Dst_simple_match: "matches (ipportiface_matcher, \<alpha>) (negation_type_to_match_expr (\<lambda>x. ipportiface_rule_match.Dst (ipv4_word_netmask_to_ipt_ipv4range x)) ip) a p \<longleftrightarrow>
+lemma matches_Dst_simple_match: "matches (ipportiface_matcher, \<alpha>) (negation_type_to_match_expr (\<lambda>x. Dst (ipv4_word_netmask_to_ipt_ipv4range x)) ip) a p \<longleftrightarrow>
   simple_match_ip ip (p_dst p)"
 apply(cases ip)
  apply(rename_tac i_ip)
@@ -95,251 +96,275 @@ subsection{*MatchExpr to Simple Match*}
 (*Unfinished*)
 text{*Unfinished*}
 
-fun ipportiface_match_to_simple_match :: "ipportiface_rule_match match_expr \<Rightarrow> simple_match" where
-  "ipportiface_match_to_simple_match (Match (IIface iif)) = simple_match_any\<lparr> iiface := iif \<rparr>" |
-  "ipportiface_match_to_simple_match (Match (OIface oif)) = simple_match_any\<lparr> oiface := oif \<rparr>" |
-  "ipportiface_match_to_simple_match (Match (Src ip)) = simple_match_any\<lparr> src := Pos (ipt_ipv4range_to_ipv4_word_netmask ip) \<rparr>" |
-  "ipportiface_match_to_simple_match (Match (Dst ip)) = simple_match_any\<lparr> dst := Pos (ipt_ipv4range_to_ipv4_word_netmask ip) \<rparr>" |
-  "ipportiface_match_to_simple_match (Match (Prot p)) = simple_match_any\<lparr> proto := p \<rparr>" |
-  "ipportiface_match_to_simple_match (Match (Src_Ports [])) = simple_match_any" |
-  "ipportiface_match_to_simple_match (Match (Src_Ports [(s,e)])) = simple_match_any\<lparr> sports := (s,e) \<rparr>" |
-  "ipportiface_match_to_simple_match (Match (Dst_Ports [])) = simple_match_any" |
-  "ipportiface_match_to_simple_match (Match (Dst_Ports [(s,e)])) = simple_match_any\<lparr> dports := (s,e) \<rparr>" |
-  "ipportiface_match_to_simple_match (MatchNot (Match (Src ip))) = simple_match_any\<lparr> src := Neg (ipt_ipv4range_to_ipv4_word_netmask ip) \<rparr>" |
-  "ipportiface_match_to_simple_match (MatchNot (Match (Dst ip))) = simple_match_any\<lparr> dst := Neg (ipt_ipv4range_to_ipv4_word_netmask ip) \<rparr>" |
+fun ipportiface_match_to_simple_match :: "ipportiface_rule_match match_expr \<Rightarrow> simple_match option" where
+  "ipportiface_match_to_simple_match MatchAny = Some simple_match_any" |
+  "ipportiface_match_to_simple_match (MatchNot MatchAny) = None" |
+  "ipportiface_match_to_simple_match (Match (IIface iif)) = Some (simple_match_any\<lparr> iiface := iif \<rparr>)" |
+  "ipportiface_match_to_simple_match (Match (OIface oif)) = Some (simple_match_any\<lparr> oiface := oif \<rparr>)" |
+  "ipportiface_match_to_simple_match (Match (Src ip)) = Some (simple_match_any\<lparr> src := Pos (ipt_ipv4range_to_ipv4_word_netmask ip) \<rparr>)" |
+  "ipportiface_match_to_simple_match (Match (Dst ip)) = Some (simple_match_any\<lparr> dst := Pos (ipt_ipv4range_to_ipv4_word_netmask ip) \<rparr>)" |
+  "ipportiface_match_to_simple_match (Match (Prot p)) = Some (simple_match_any\<lparr> proto := p \<rparr>)" |
+  "ipportiface_match_to_simple_match (Match (Src_Ports [])) = Some (simple_match_any)" |
+  "ipportiface_match_to_simple_match (Match (Src_Ports [(s,e)])) = Some (simple_match_any\<lparr> sports := (s,e) \<rparr>)" |
+  "ipportiface_match_to_simple_match (Match (Dst_Ports [])) = Some (simple_match_any)" |
+  "ipportiface_match_to_simple_match (Match (Dst_Ports [(s,e)])) = Some (simple_match_any\<lparr> dports := (s,e) \<rparr>)" |
+  "ipportiface_match_to_simple_match (MatchNot (Match (Src ip))) = Some (simple_match_any\<lparr> src := Neg (ipt_ipv4range_to_ipv4_word_netmask ip) \<rparr>)" |
+  "ipportiface_match_to_simple_match (MatchNot (Match (Dst ip))) = Some (simple_match_any\<lparr> dst := Neg (ipt_ipv4range_to_ipv4_word_netmask ip) \<rparr>)" |
+  "ipportiface_match_to_simple_match (MatchNot (Match (IIface IfaceAny))) = None" |
+  "ipportiface_match_to_simple_match (MatchNot (Match (IIface (Iface (Pos eth))))) = Some (simple_match_any\<lparr> iiface := Iface (Neg eth) \<rparr>)" |
+  "ipportiface_match_to_simple_match (MatchNot (Match (IIface (Iface (Neg eth))))) = Some (simple_match_any\<lparr> iiface := Iface (Pos eth) \<rparr>)" |
+  "ipportiface_match_to_simple_match (MatchNot (Match (OIface IfaceAny))) = None" |
+  "ipportiface_match_to_simple_match (MatchNot (Match (OIface (Iface (Pos eth))))) = Some (simple_match_any\<lparr> oiface := Iface (Neg eth) \<rparr>)" |
+  "ipportiface_match_to_simple_match (MatchNot (Match (OIface (Iface (Neg eth))))) = Some (simple_match_any\<lparr> oiface := Iface (Pos eth) \<rparr>)" |
+  "ipportiface_match_to_simple_match (MatchNot (Match (Prot ProtoAny))) = None" |
+  "ipportiface_match_to_simple_match (MatchNot (Match (Prot (Proto (Pos p))))) =  Some (simple_match_any\<lparr> proto := Proto (Neg p) \<rparr>)" |
+  "ipportiface_match_to_simple_match (MatchNot (Match (Prot (Proto (Neg p))))) =  Some (simple_match_any\<lparr> proto := Proto (Pos p) \<rparr>)" |
   --"undefined cases, normalize before!"
+  "ipportiface_match_to_simple_match (MatchNot (MatchAnd _ _)) = undefined" |
+  "ipportiface_match_to_simple_match (MatchNot (MatchNot _)) = undefined" |
   "ipportiface_match_to_simple_match (Match (Src_Ports (_#_))) = undefined" |
   "ipportiface_match_to_simple_match (Match (Dst_Ports (_#_))) = undefined" |
-  "ipportiface_match_to_simple_match (Match (Extra _)) = undefined"
-  (* hmm, port list (\<or>) to one port, creates multiple rules! need normalize_ports for match_Expr*)
+  "ipportiface_match_to_simple_match (MatchNot (Match (Src_Ports _))) = undefined" |
+  "ipportiface_match_to_simple_match (MatchNot (Match (Dst_Ports _))) = undefined" |
+  "ipportiface_match_to_simple_match (Match (Extra _)) = undefined" |
+  "ipportiface_match_to_simple_match (MatchNot (Match (Extra _))) = undefined"
 (*\<dots>*)
 
+subsubsection{*Merging Simple Matches*}
+text{*@{typ "simple_match"} @{text \<and>} @{typ "simple_match"}*}
 
-
-(*TODO: Move?*)
-fun ipt_ports_negation_type_normalize :: "ipt_ports negation_type \<Rightarrow> ipt_ports" where
-  "ipt_ports_negation_type_normalize (Pos ps) = ps" |
-  "ipt_ports_negation_type_normalize (Neg ps) = br2l (bitrange_invert (l2br ps))"
-
-
-
-(*warning!! an empty port range means it can never match! no port range matches (corresponds to firewall behavior, but usually you cannot specify an empty portrange here)*)
-lemma "ipt_ports_negation_type_normalize (Neg [(0,65535)]) = []" by eval
-lemma "\<not> matches (ipportiface_matcher, \<alpha>) (MatchNot (Match (Src_Ports [(0,65535)]))) a 
-        \<lparr>p_iiface = ''eth0'', p_oiface = ''eth1'', p_src = ipv4addr_of_dotteddecimal (192,168,2,45), p_dst= ipv4addr_of_dotteddecimal (173,194,112,111),
-                 p_proto=TCP, p_sport=2065, p_dport=80\<rparr>"
-by(simp add: matches_case_ternaryvalue_tuple split: ternaryvalue.split)
-lemma "matches (ipportiface_matcher, \<alpha>) (MatchNot (Match (Src_Ports []))) a 
-        \<lparr>p_iiface = ''eth0'', p_oiface = ''eth1'', p_src = ipv4addr_of_dotteddecimal (192,168,2,45), p_dst= ipv4addr_of_dotteddecimal (173,194,112,111),
-                 p_proto=TCP, p_sport=2065, p_dport=80\<rparr>"
-by(simp add: matches_case_ternaryvalue_tuple split: ternaryvalue.split)
-lemma "\<not>matches (ipportiface_matcher, \<alpha>) (MatchNot (Match (Src_Ports [(1024,4096)]))) a 
-        \<lparr>p_iiface = ''eth0'', p_oiface = ''eth1'', p_src = ipv4addr_of_dotteddecimal (192,168,2,45), p_dst= ipv4addr_of_dotteddecimal (173,194,112,111),
-                 p_proto=TCP, p_sport=2065, p_dport=80\<rparr>"
-by(simp add: matches_case_ternaryvalue_tuple split: ternaryvalue.split)
-
-
-
-declare ipt_ports_negation_type_normalize.simps[simp del]
-
-lemma ipt_ports_negation_type_normalize_correct:
-      "matches (ipportiface_matcher, \<alpha>) (negation_type_to_match_expr (Src_Ports) ps) a p \<longleftrightarrow>
-       matches (ipportiface_matcher, \<alpha>) (Match (Src_Ports (ipt_ports_negation_type_normalize ps))) a p"
-      "matches (ipportiface_matcher, \<alpha>) (negation_type_to_match_expr (Dst_Ports) ps) a p \<longleftrightarrow>
-       matches (ipportiface_matcher, \<alpha>) (Match (Dst_Ports (ipt_ports_negation_type_normalize ps))) a p"
-apply(case_tac [!] ps)
-apply(simp_all add: ipt_ports_negation_type_normalize.simps matches_case_ternaryvalue_tuple bunch_of_lemmata_about_matches bool_to_ternary_simps l2br_br2l ports_to_set_bitrange split: ternaryvalue.split)
-done
-
-(*todo: move*)
-value "primitive_extractor (is_Src_Ports, src_ports_sel) m"
-
-term fold
-(* [ [(1,2) \<or> (3,4)]  \<and>  [] ]*)
-definition ipt_ports_andlist_compress :: "ipt_ports list \<Rightarrow> ipt_ports" where
-  "ipt_ports_andlist_compress pss = br2l (fold (\<lambda>ps accu. (bitrange_intersection (l2br ps) accu)) pss bitrange_UNIV)"
-
-lemma ipt_ports_andlist_compress_correct: "ports_to_set (ipt_ports_andlist_compress pss) = \<Inter> set (map ports_to_set pss)"
-  proof -
-    { fix accu
-      have "ports_to_set (br2l (fold (\<lambda>ps accu. (bitrange_intersection (l2br ps) accu)) pss accu)) = (\<Inter> set (map ports_to_set pss)) \<inter> (ports_to_set (br2l accu))"
-        apply(induction pss arbitrary: accu)
-         apply(simp_all add: ports_to_set_bitrange l2br_br2l)
-        by fast
-    }
-    from this[of bitrange_UNIV] show ?thesis
-      unfolding ipt_ports_andlist_compress_def by(simp add: ports_to_set_bitrange l2br_br2l)
+subsubsection{*Normalizing ports*}
+  
+  (*TODO: Move?*)
+  fun ipt_ports_negation_type_normalize :: "ipt_ports negation_type \<Rightarrow> ipt_ports" where
+    "ipt_ports_negation_type_normalize (Pos ps) = ps" |
+    "ipt_ports_negation_type_normalize (Neg ps) = br2l (bitrange_invert (l2br ps))"
+  
+  
+  
+  (*warning!! an empty port range means it can never match!
+    No port range matches (corresponds to firewall behavior, but usually you cannot specify an empty portrange here)*)
+  lemma "ipt_ports_negation_type_normalize (Neg [(0,65535)]) = []" by eval
+  lemma "\<not> matches (ipportiface_matcher, \<alpha>) (MatchNot (Match (Src_Ports [(0,65535)]))) a 
+          \<lparr>p_iiface = ''eth0'', p_oiface = ''eth1'', p_src = ipv4addr_of_dotteddecimal (192,168,2,45), p_dst= ipv4addr_of_dotteddecimal (173,194,112,111),
+                   p_proto=TCP, p_sport=2065, p_dport=80\<rparr>"
+  by(simp add: matches_case_ternaryvalue_tuple split: ternaryvalue.split)
+  lemma "matches (ipportiface_matcher, \<alpha>) (MatchNot (Match (Src_Ports []))) a 
+          \<lparr>p_iiface = ''eth0'', p_oiface = ''eth1'', p_src = ipv4addr_of_dotteddecimal (192,168,2,45), p_dst= ipv4addr_of_dotteddecimal (173,194,112,111),
+                   p_proto=TCP, p_sport=2065, p_dport=80\<rparr>"
+  by(simp add: matches_case_ternaryvalue_tuple split: ternaryvalue.split)
+  lemma "\<not>matches (ipportiface_matcher, \<alpha>) (MatchNot (Match (Src_Ports [(1024,4096)]))) a 
+          \<lparr>p_iiface = ''eth0'', p_oiface = ''eth1'', p_src = ipv4addr_of_dotteddecimal (192,168,2,45), p_dst= ipv4addr_of_dotteddecimal (173,194,112,111),
+                   p_proto=TCP, p_sport=2065, p_dport=80\<rparr>"
+  by(simp add: matches_case_ternaryvalue_tuple split: ternaryvalue.split)
+  
+  
+  
+  declare ipt_ports_negation_type_normalize.simps[simp del]
+  
+  lemma ipt_ports_negation_type_normalize_correct:
+        "matches (ipportiface_matcher, \<alpha>) (negation_type_to_match_expr (Src_Ports) ps) a p \<longleftrightarrow>
+         matches (ipportiface_matcher, \<alpha>) (Match (Src_Ports (ipt_ports_negation_type_normalize ps))) a p"
+        "matches (ipportiface_matcher, \<alpha>) (negation_type_to_match_expr (Dst_Ports) ps) a p \<longleftrightarrow>
+         matches (ipportiface_matcher, \<alpha>) (Match (Dst_Ports (ipt_ports_negation_type_normalize ps))) a p"
+  apply(case_tac [!] ps)
+  apply(simp_all add: ipt_ports_negation_type_normalize.simps matches_case_ternaryvalue_tuple
+          bunch_of_lemmata_about_matches bool_to_ternary_simps l2br_br2l ports_to_set_bitrange split: ternaryvalue.split)
+  done
+  
+  (* [ [(1,2) \<or> (3,4)]  \<and>  [] ]*)
+  definition ipt_ports_andlist_compress :: "ipt_ports list \<Rightarrow> ipt_ports" where
+    "ipt_ports_andlist_compress pss = br2l (fold (\<lambda>ps accu. (bitrange_intersection (l2br ps) accu)) pss bitrange_UNIV)"
+  
+  lemma ipt_ports_andlist_compress_correct: "ports_to_set (ipt_ports_andlist_compress pss) = \<Inter> set (map ports_to_set pss)"
+    proof -
+      { fix accu
+        have "ports_to_set (br2l (fold (\<lambda>ps accu. (bitrange_intersection (l2br ps) accu)) pss accu)) = (\<Inter> set (map ports_to_set pss)) \<inter> (ports_to_set (br2l accu))"
+          apply(induction pss arbitrary: accu)
+           apply(simp_all add: ports_to_set_bitrange l2br_br2l)
+          by fast
+      }
+      from this[of bitrange_UNIV] show ?thesis
+        unfolding ipt_ports_andlist_compress_def by(simp add: ports_to_set_bitrange l2br_br2l)
+    qed
+  
+  
+  definition ipt_ports_compress :: "ipt_ports negation_type list \<Rightarrow> ipt_ports" where
+    "ipt_ports_compress pss = ipt_ports_andlist_compress (map ipt_ports_negation_type_normalize pss)"
+  
+  
+  (*TODO: only for src*)
+  lemma ipt_ports_compress_src_correct:
+    "matches (ipportiface_matcher, \<alpha>) (alist_and (NegPos_map Src_Ports ms)) a p \<longleftrightarrow> matches (ipportiface_matcher, \<alpha>) (Match (Src_Ports (ipt_ports_compress ms))) a p"
+  proof(induction ms)
+    case Nil thus ?case by(simp add: ipt_ports_compress_def bunch_of_lemmata_about_matches ipt_ports_andlist_compress_correct)
+    next
+    case (Cons m ms)
+      thus ?case (is ?goal)
+      proof(cases m)
+        case Pos thus ?goal using Cons.IH
+          by(simp add: ipt_ports_compress_def ipt_ports_andlist_compress_correct bunch_of_lemmata_about_matches
+              ternary_to_bool_bool_to_ternary ipt_ports_negation_type_normalize.simps)
+        next
+        case (Neg a)
+          thus ?goal using Cons.IH
+          apply(simp add: ipt_ports_compress_def ipt_ports_andlist_compress_correct bunch_of_lemmata_about_matches ternary_to_bool_bool_to_ternary)
+          apply(simp add: matches_case_ternaryvalue_tuple bool_to_ternary_simps l2br_br2l
+                  ports_to_set_bitrange ipt_ports_negation_type_normalize.simps split: ternaryvalue.split)
+          done
+        qed
   qed
-
-
-definition ipt_ports_compress :: "ipt_ports negation_type list \<Rightarrow> ipt_ports" where
-  "ipt_ports_compress pss = ipt_ports_andlist_compress (map ipt_ports_negation_type_normalize pss)"
-
-
-(*TODO: only for src*)
-lemma ipt_ports_compress_src_correct:
-  "matches (ipportiface_matcher, \<alpha>) (alist_and (NegPos_map Src_Ports ms)) a p \<longleftrightarrow> matches (ipportiface_matcher, \<alpha>) (Match (Src_Ports (ipt_ports_compress ms))) a p"
-proof(induction ms)
-  case Nil thus ?case by(simp add: ipt_ports_compress_def bunch_of_lemmata_about_matches ipt_ports_andlist_compress_correct)
-  next
-  case (Cons m ms)
-    thus ?case (is ?goal)
-    proof(cases m)
-      case Pos thus ?goal using Cons.IH
-        by(simp add: ipt_ports_compress_def ipt_ports_andlist_compress_correct bunch_of_lemmata_about_matches ternary_to_bool_bool_to_ternary ipt_ports_negation_type_normalize.simps)
-      next
-      case (Neg a)
-        thus ?goal using Cons.IH
-        apply(simp add: ipt_ports_compress_def ipt_ports_andlist_compress_correct bunch_of_lemmata_about_matches ternary_to_bool_bool_to_ternary)
-        apply(simp add: matches_case_ternaryvalue_tuple bool_to_ternary_simps l2br_br2l ports_to_set_bitrange ipt_ports_negation_type_normalize.simps split: ternaryvalue.split)
-        done
-      qed
-qed
-lemma ipt_ports_compress_dst_correct:
-  "matches (ipportiface_matcher, \<alpha>) (alist_and (NegPos_map Dst_Ports ms)) a p \<longleftrightarrow> matches (ipportiface_matcher, \<alpha>) (Match (Dst_Ports (ipt_ports_compress ms))) a p"
-proof(induction ms)
-  case Nil thus ?case by(simp add: ipt_ports_compress_def bunch_of_lemmata_about_matches ipt_ports_andlist_compress_correct)
-  next
-  case (Cons m ms)
-    thus ?case (is ?goal)
-    proof(cases m)
-      case Pos thus ?goal using Cons.IH
-        by(simp add: ipt_ports_compress_def ipt_ports_andlist_compress_correct bunch_of_lemmata_about_matches ternary_to_bool_bool_to_ternary ipt_ports_negation_type_normalize.simps)
-      next
-      case (Neg a)
-        thus ?goal using Cons.IH
-        apply(simp add: ipt_ports_compress_def ipt_ports_andlist_compress_correct bunch_of_lemmata_about_matches ternary_to_bool_bool_to_ternary)
-        apply(simp add: matches_case_ternaryvalue_tuple bool_to_ternary_simps l2br_br2l ports_to_set_bitrange ipt_ports_negation_type_normalize.simps split: ternaryvalue.split)
-        done
-      qed
-qed
-
-
-lemma ipt_ports_compress_matches_set: "matches (ipportiface_matcher, \<alpha>) (Match (Src_Ports (ipt_ports_compress ips))) a p \<longleftrightarrow>
-       p_sport p \<in> \<Inter> set (map (ports_to_set \<circ> ipt_ports_negation_type_normalize) ips)"
-apply(simp add: ipt_ports_compress_def)
-apply(induction ips)
- apply(simp)
- apply(simp add: ipt_ports_compress_def bunch_of_lemmata_about_matches ipt_ports_andlist_compress_correct)
-apply(rename_tac m ms)
-apply(case_tac m)
- apply(simp add: ipt_ports_andlist_compress_correct bunch_of_lemmata_about_matches ternary_to_bool_bool_to_ternary ipt_ports_negation_type_normalize.simps)
-apply(simp add: ipt_ports_andlist_compress_correct bunch_of_lemmata_about_matches ternary_to_bool_bool_to_ternary)
-done
-
-
-(*spliting the primitives: multiport list (a list of disjunction!)*)
-lemma singletonize_SrcDst_Ports: "match_list (ipportiface_matcher, \<alpha>) (map (\<lambda>spt. (MatchAnd (Match (Src_Ports [spt]))) ms) (spts)) a p \<longleftrightarrow>
-       matches (ipportiface_matcher, \<alpha>) (MatchAnd (Match (Src_Ports spts)) ms) a p"
-       "match_list (ipportiface_matcher, \<alpha>) (map (\<lambda>spt. (MatchAnd (Match (Dst_Ports [spt]))) ms) (dpts)) a p \<longleftrightarrow>
-       matches (ipportiface_matcher, \<alpha>) (MatchAnd (Match (Dst_Ports dpts)) ms) a p"
-  apply(simp_all add: match_list_matches bunch_of_lemmata_about_matches(1) multiports_disjuction)
-done
-
-
-(*idea:*)
-value "case primitive_extractor (is_Src_Ports, src_ports_sel) m 
-        of (spts, rst) \<Rightarrow> map (\<lambda>spt. (MatchAnd (Match (Src_Ports [spt]))) rst) (ipt_ports_compress spts)"
-
-
-text{*Normalizing match expressions such that at most one port will exist in it. Returns a list of match expressions (splits one firewall rule into several rules).*}
-definition normalize_ports_step :: "((ipportiface_rule_match \<Rightarrow> bool) \<times> (ipportiface_rule_match \<Rightarrow> ipt_ports)) \<Rightarrow> 
-                             (ipt_ports \<Rightarrow> ipportiface_rule_match) \<Rightarrow>
-                             ipportiface_rule_match match_expr \<Rightarrow> ipportiface_rule_match match_expr list" where 
-  "normalize_ports_step (disc_sel) C  m = (case primitive_extractor (disc_sel) m 
-              of (spts, rst) \<Rightarrow> map (\<lambda>spt. (MatchAnd (Match (C [spt]))) rst) (ipt_ports_compress spts))"
-
-
-lemma normalize_ports_step_Src: assumes "normalized_match m" shows
-      "match_list (ipportiface_matcher, \<alpha>) (normalize_ports_step (is_Src_Ports, src_ports_sel) Src_Ports m) a p \<longleftrightarrow>
-       matches (ipportiface_matcher, \<alpha>) m a p"
-  proof -
-    obtain as ms where pe: "primitive_extractor (is_Src_Ports, src_ports_sel) m = (as, ms)" by fastforce
-    from pe have normalize_ports_step: "normalize_ports_step (is_Src_Ports, src_ports_sel) Src_Ports m = (map (\<lambda>spt. MatchAnd (Match (Src_Ports [spt])) ms) (ipt_ports_compress as))"
-      by(simp add: normalize_ports_step_def)
-    from pe  primitive_extractor_correct(1)[OF assms wf_disc_sel_ipportiface_rule_match(1), where \<gamma>="(ipportiface_matcher, \<alpha>)" and a=a and p=p] have 
-      "matches (ipportiface_matcher, \<alpha>) m a p \<longleftrightarrow> (matches (ipportiface_matcher, \<alpha>) (alist_and (NegPos_map Src_Ports as)) a p \<and> matches (ipportiface_matcher, \<alpha>) ms a p)"
-    by simp
-    also have "... \<longleftrightarrow> match_list (ipportiface_matcher, \<alpha>) (normalize_ports_step (is_Src_Ports, src_ports_sel) Src_Ports m) a p"
-      by(simp add: normalize_ports_step singletonize_SrcDst_Ports(1) bunch_of_lemmata_about_matches(1) ipt_ports_compress_src_correct)
-    finally show ?thesis by simp
+  lemma ipt_ports_compress_dst_correct:
+    "matches (ipportiface_matcher, \<alpha>) (alist_and (NegPos_map Dst_Ports ms)) a p \<longleftrightarrow> matches (ipportiface_matcher, \<alpha>) (Match (Dst_Ports (ipt_ports_compress ms))) a p"
+  proof(induction ms)
+    case Nil thus ?case by(simp add: ipt_ports_compress_def bunch_of_lemmata_about_matches ipt_ports_andlist_compress_correct)
+    next
+    case (Cons m ms)
+      thus ?case (is ?goal)
+      proof(cases m)
+        case Pos thus ?goal using Cons.IH
+          by(simp add: ipt_ports_compress_def ipt_ports_andlist_compress_correct bunch_of_lemmata_about_matches
+                ternary_to_bool_bool_to_ternary ipt_ports_negation_type_normalize.simps)
+        next
+        case (Neg a)
+          thus ?goal using Cons.IH
+          apply(simp add: ipt_ports_compress_def ipt_ports_andlist_compress_correct bunch_of_lemmata_about_matches ternary_to_bool_bool_to_ternary)
+          apply(simp add: matches_case_ternaryvalue_tuple bool_to_ternary_simps l2br_br2l ports_to_set_bitrange
+              ipt_ports_negation_type_normalize.simps split: ternaryvalue.split)
+          done
+        qed
   qed
-lemma normalize_ports_step_Dst: assumes "normalized_match m" shows
-      "match_list (ipportiface_matcher, \<alpha>) (normalize_ports_step (is_Dst_Ports, dst_ports_sel) Dst_Ports m) a p \<longleftrightarrow>
-       matches (ipportiface_matcher, \<alpha>) m a p"
-  proof -
-    obtain as ms where pe: "primitive_extractor (is_Dst_Ports, dst_ports_sel) m = (as, ms)" by fastforce
-    from pe have normalize_ports_step: "normalize_ports_step (is_Dst_Ports, dst_ports_sel) Dst_Ports m = (map (\<lambda>spt. MatchAnd (Match (Dst_Ports [spt])) ms) (ipt_ports_compress as))"
-      by(simp add: normalize_ports_step_def)
-    from pe  primitive_extractor_correct(1)[OF assms wf_disc_sel_ipportiface_rule_match(2), where \<gamma>="(ipportiface_matcher, \<alpha>)" and a=a and p=p] have 
-      "matches (ipportiface_matcher, \<alpha>) m a p \<longleftrightarrow> (matches (ipportiface_matcher, \<alpha>) (alist_and (NegPos_map Dst_Ports as)) a p \<and> matches (ipportiface_matcher, \<alpha>) ms a p)"
-    by simp
-    also have "... \<longleftrightarrow> match_list (ipportiface_matcher, \<alpha>) (normalize_ports_step (is_Dst_Ports, dst_ports_sel) Dst_Ports m) a p"
-      by(simp add: normalize_ports_step singletonize_SrcDst_Ports(2) bunch_of_lemmata_about_matches(1) ipt_ports_compress_dst_correct)
-    finally show ?thesis by simp
-  qed
-
-
-fun normalized_src_ports :: "ipportiface_rule_match match_expr \<Rightarrow> bool" where
-  "normalized_src_ports MatchAny = True" |
-  "normalized_src_ports (Match (Src_Ports [])) = True" |
-  "normalized_src_ports (Match (Src_Ports [_])) = True" |
-  "normalized_src_ports (Match (Src_Ports _)) = False" |
-  "normalized_src_ports (Match _) = True" |
-  "normalized_src_ports (MatchNot (Match (Src_Ports _))) = False" |
-  "normalized_src_ports (MatchAnd m1 m2) = (normalized_src_ports m1 \<and> normalized_src_ports m2)" |
-  "normalized_src_ports (MatchNot (MatchAnd _ _)) = False" |
-  "normalized_src_ports (MatchNot _) = True"
-
-fun normalized_dst_ports :: "ipportiface_rule_match match_expr \<Rightarrow> bool" where
-  "normalized_dst_ports MatchAny = True" |
-  "normalized_dst_ports (Match (Dst_Ports [])) = True" |
-  "normalized_dst_ports (Match (Dst_Ports [_])) = True" |
-  "normalized_dst_ports (Match (Dst_Ports _)) = False" |
-  "normalized_dst_ports (Match _) = True" |
-  "normalized_dst_ports (MatchNot (Match (Dst_Ports _))) = False" |
-  "normalized_dst_ports (MatchAnd m1 m2) = (normalized_dst_ports m1 \<and> normalized_dst_ports m2)" |
-  "normalized_dst_ports (MatchNot (MatchAnd _ _)) = False" |
-  "normalized_dst_ports (MatchNot _) = True" 
-
-lemma normalized_match_MatchNot_D: "normalized_match (MatchNot m) \<Longrightarrow> normalized_match m"
-apply(induction m)
-apply(simp_all)
-done
-
-
-lemma "\<forall>spt \<in> set (ipt_ports_compress spts). normalized_src_ports (Match (Src_Ports [spt]))" by(simp)
-
-lemma help1: "normalized_match ms \<Longrightarrow> \<not> has_disc is_Src_Ports ms \<Longrightarrow> normalized_src_ports ms"
-  apply(induction ms rule: normalized_src_ports.induct)
+  
+  
+  lemma ipt_ports_compress_matches_set: "matches (ipportiface_matcher, \<alpha>) (Match (Src_Ports (ipt_ports_compress ips))) a p \<longleftrightarrow>
+         p_sport p \<in> \<Inter> set (map (ports_to_set \<circ> ipt_ports_negation_type_normalize) ips)"
+  apply(simp add: ipt_ports_compress_def)
+  apply(induction ips)
+   apply(simp)
+   apply(simp add: ipt_ports_compress_def bunch_of_lemmata_about_matches ipt_ports_andlist_compress_correct)
+  apply(rename_tac m ms)
+  apply(case_tac m)
+   apply(simp add: ipt_ports_andlist_compress_correct bunch_of_lemmata_about_matches ternary_to_bool_bool_to_ternary ipt_ports_negation_type_normalize.simps)
+  apply(simp add: ipt_ports_andlist_compress_correct bunch_of_lemmata_about_matches ternary_to_bool_bool_to_ternary)
+  done
+  
+  
+  (*spliting the primitives: multiport list (a list of disjunction!)*)
+  lemma singletonize_SrcDst_Ports: "match_list (ipportiface_matcher, \<alpha>) (map (\<lambda>spt. (MatchAnd (Match (Src_Ports [spt]))) ms) (spts)) a p \<longleftrightarrow>
+         matches (ipportiface_matcher, \<alpha>) (MatchAnd (Match (Src_Ports spts)) ms) a p"
+         "match_list (ipportiface_matcher, \<alpha>) (map (\<lambda>spt. (MatchAnd (Match (Dst_Ports [spt]))) ms) (dpts)) a p \<longleftrightarrow>
+         matches (ipportiface_matcher, \<alpha>) (MatchAnd (Match (Dst_Ports dpts)) ms) a p"
+    apply(simp_all add: match_list_matches bunch_of_lemmata_about_matches(1) multiports_disjuction)
+  done
+  
+  
+  (*idea:*)
+  value "case primitive_extractor (is_Src_Ports, src_ports_sel) m 
+          of (spts, rst) \<Rightarrow> map (\<lambda>spt. (MatchAnd (Match (Src_Ports [spt]))) rst) (ipt_ports_compress spts)"
+  
+  
+  text{*Normalizing match expressions such that at most one port will exist in it. Returns a list of match expressions (splits one firewall rule into several rules).*}
+  definition normalize_ports_step :: "((ipportiface_rule_match \<Rightarrow> bool) \<times> (ipportiface_rule_match \<Rightarrow> ipt_ports)) \<Rightarrow> 
+                               (ipt_ports \<Rightarrow> ipportiface_rule_match) \<Rightarrow>
+                               ipportiface_rule_match match_expr \<Rightarrow> ipportiface_rule_match match_expr list" where 
+    "normalize_ports_step (disc_sel) C  m = (case primitive_extractor (disc_sel) m 
+                of (spts, rst) \<Rightarrow> map (\<lambda>spt. (MatchAnd (Match (C [spt]))) rst) (ipt_ports_compress spts))"
+  
+  
+  lemma normalize_ports_step_Src: assumes "normalized_match m" shows
+        "match_list (ipportiface_matcher, \<alpha>) (normalize_ports_step (is_Src_Ports, src_ports_sel) Src_Ports m) a p \<longleftrightarrow>
+         matches (ipportiface_matcher, \<alpha>) m a p"
+    proof -
+      obtain as ms where pe: "primitive_extractor (is_Src_Ports, src_ports_sel) m = (as, ms)" by fastforce
+      from pe have normalize_ports_step: "normalize_ports_step (is_Src_Ports, src_ports_sel) Src_Ports m = 
+            (map (\<lambda>spt. MatchAnd (Match (Src_Ports [spt])) ms) (ipt_ports_compress as))"
+        by(simp add: normalize_ports_step_def)
+      from pe  primitive_extractor_correct(1)[OF assms wf_disc_sel_ipportiface_rule_match(1), where \<gamma>="(ipportiface_matcher, \<alpha>)" and a=a and p=p] have 
+        "matches (ipportiface_matcher, \<alpha>) m a p \<longleftrightarrow> 
+          (matches (ipportiface_matcher, \<alpha>) (alist_and (NegPos_map Src_Ports as)) a p \<and> matches (ipportiface_matcher, \<alpha>) ms a p)"
+      by simp
+      also have "... \<longleftrightarrow> match_list (ipportiface_matcher, \<alpha>) (normalize_ports_step (is_Src_Ports, src_ports_sel) Src_Ports m) a p"
+        by(simp add: normalize_ports_step singletonize_SrcDst_Ports(1) bunch_of_lemmata_about_matches(1) ipt_ports_compress_src_correct)
+      finally show ?thesis by simp
+    qed
+  lemma normalize_ports_step_Dst: assumes "normalized_match m" shows
+        "match_list (ipportiface_matcher, \<alpha>) (normalize_ports_step (is_Dst_Ports, dst_ports_sel) Dst_Ports m) a p \<longleftrightarrow>
+         matches (ipportiface_matcher, \<alpha>) m a p"
+    proof -
+      obtain as ms where pe: "primitive_extractor (is_Dst_Ports, dst_ports_sel) m = (as, ms)" by fastforce
+      from pe have normalize_ports_step: "normalize_ports_step (is_Dst_Ports, dst_ports_sel) Dst_Ports m =
+          (map (\<lambda>spt. MatchAnd (Match (Dst_Ports [spt])) ms) (ipt_ports_compress as))"
+        by(simp add: normalize_ports_step_def)
+      from pe  primitive_extractor_correct(1)[OF assms wf_disc_sel_ipportiface_rule_match(2), where \<gamma>="(ipportiface_matcher, \<alpha>)" and a=a and p=p] have 
+        "matches (ipportiface_matcher, \<alpha>) m a p \<longleftrightarrow>
+          (matches (ipportiface_matcher, \<alpha>) (alist_and (NegPos_map Dst_Ports as)) a p \<and> matches (ipportiface_matcher, \<alpha>) ms a p)"
+      by simp
+      also have "... \<longleftrightarrow> match_list (ipportiface_matcher, \<alpha>) (normalize_ports_step (is_Dst_Ports, dst_ports_sel) Dst_Ports m) a p"
+        by(simp add: normalize_ports_step singletonize_SrcDst_Ports(2) bunch_of_lemmata_about_matches(1) ipt_ports_compress_dst_correct)
+      finally show ?thesis by simp
+    qed
+  
+  
+  fun normalized_src_ports :: "ipportiface_rule_match match_expr \<Rightarrow> bool" where
+    "normalized_src_ports MatchAny = True" |
+    "normalized_src_ports (Match (Src_Ports [])) = True" |
+    "normalized_src_ports (Match (Src_Ports [_])) = True" |
+    "normalized_src_ports (Match (Src_Ports _)) = False" |
+    "normalized_src_ports (Match _) = True" |
+    "normalized_src_ports (MatchNot (Match (Src_Ports _))) = False" |
+    "normalized_src_ports (MatchAnd m1 m2) = (normalized_src_ports m1 \<and> normalized_src_ports m2)" |
+    "normalized_src_ports (MatchNot (MatchAnd _ _)) = False" |
+    "normalized_src_ports (MatchNot _) = True"
+  
+  fun normalized_dst_ports :: "ipportiface_rule_match match_expr \<Rightarrow> bool" where
+    "normalized_dst_ports MatchAny = True" |
+    "normalized_dst_ports (Match (Dst_Ports [])) = True" |
+    "normalized_dst_ports (Match (Dst_Ports [_])) = True" |
+    "normalized_dst_ports (Match (Dst_Ports _)) = False" |
+    "normalized_dst_ports (Match _) = True" |
+    "normalized_dst_ports (MatchNot (Match (Dst_Ports _))) = False" |
+    "normalized_dst_ports (MatchAnd m1 m2) = (normalized_dst_ports m1 \<and> normalized_dst_ports m2)" |
+    "normalized_dst_ports (MatchNot (MatchAnd _ _)) = False" |
+    "normalized_dst_ports (MatchNot _) = True" 
+  
+  lemma normalized_match_MatchNot_D: "normalized_match (MatchNot m) \<Longrightarrow> normalized_match m"
+  apply(induction m)
   apply(simp_all)
   done
-
-lemma normalize_ports_step_normalized_src_ports_helper: "normalized_match m \<Longrightarrow> 
-      primitive_extractor (is_Src_Ports, src_ports_sel) m = (spts, ms) \<Longrightarrow>
-      ml \<in> set (map (\<lambda>spt. (MatchAnd (Match (Src_Ports [spt]))) ms) (ipt_ports_compress spts))\<Longrightarrow>
-      normalized_src_ports ml"
-apply(simp)
-apply(frule(1) primitive_extractor_correct(2)[OF _ wf_disc_sel_ipportiface_rule_match(1)])
-apply(frule(1) primitive_extractor_correct(3)[OF _ wf_disc_sel_ipportiface_rule_match(1)])
-apply(simp add: ipt_ports_compress_def)
-apply(drule(1) help1)
-apply(induction spts)
- apply(clarsimp)+
-done
-
-lemma "normalized_match m \<Longrightarrow> \<forall>mn \<in> set (normalize_ports_step (is_Src_Ports, src_ports_sel) Src_Ports m). normalized_src_ports mn \<and> normalized_match mn"
-  unfolding normalize_ports_step_def
-  apply(simp)
-  apply(intro allI impI)
-  apply(elim exE)
-  apply(rename_tac ms pts)
-  apply(rule conjI)
-   using normalize_ports_step_normalized_src_ports_helper apply(force)
-  apply(drule_tac as=pts and ms=ms in primitive_extractor_correct(2)[OF _ wf_disc_sel_ipportiface_rule_match(1)])
-   apply(simp)
-  by fastforce
   
+  
+  lemma "\<forall>spt \<in> set (ipt_ports_compress spts). normalized_src_ports (Match (Src_Ports [spt]))" by(simp)
+  
+  lemma help1: "normalized_match ms \<Longrightarrow> \<not> has_disc is_Src_Ports ms \<Longrightarrow> normalized_src_ports ms"
+    apply(induction ms rule: normalized_src_ports.induct)
+    apply(simp_all)
+    done
+  
+  lemma normalize_ports_step_normalized_src_ports_helper: "normalized_match m \<Longrightarrow> 
+        primitive_extractor (is_Src_Ports, src_ports_sel) m = (spts, ms) \<Longrightarrow>
+        ml \<in> set (map (\<lambda>spt. (MatchAnd (Match (Src_Ports [spt]))) ms) (ipt_ports_compress spts))\<Longrightarrow>
+        normalized_src_ports ml"
+  apply(simp)
+  apply(frule(1) primitive_extractor_correct(2)[OF _ wf_disc_sel_ipportiface_rule_match(1)])
+  apply(frule(1) primitive_extractor_correct(3)[OF _ wf_disc_sel_ipportiface_rule_match(1)])
+  apply(simp add: ipt_ports_compress_def)
+  apply(drule(1) help1)
+  apply(induction spts)
+   apply(clarsimp)+
+  done
+  
+  lemma "normalized_match m \<Longrightarrow> \<forall>mn \<in> set (normalize_ports_step (is_Src_Ports, src_ports_sel) Src_Ports m). normalized_src_ports mn \<and> normalized_match mn"
+    unfolding normalize_ports_step_def
+    apply(simp)
+    apply(intro allI impI)
+    apply(elim exE)
+    apply(rename_tac ms pts)
+    apply(rule conjI)
+     using normalize_ports_step_normalized_src_ports_helper apply(force)
+    apply(drule_tac as=pts and ms=ms in primitive_extractor_correct(2)[OF _ wf_disc_sel_ipportiface_rule_match(1)])
+     apply(simp)
+    by fastforce
+    
 
 
 end
